sync

LearnLean4/04.lean
@@ -4,12 +4,87 @@ namespace Equality
 #check Eq.refl
 #check Eq.symm
 
+
+def proofEqA (a : α) := Eq.refl a
+#check proofEqA
+
 variable (p q : Prop)
 
-def eq1 : Prop := p = p
-def h : (eq1 p) := Eq.refl p
+def h1 := p ∨ q
+def h2 := Eq.refl p
+def h3 (h₁ : p = q) := Eq.symm h₁
+def h4 (h₁ : p ∧ q) := And.symm h₁
+
+#check h3
+#check h4
+
 
 def p0 (a : α): Prop := a = a
 def p1 (a: α) (b: α) : Prop := a = b
-def h1 (h: p1 a b) : (b=a) := Eq.symm h
+theorem h10 (h: p1 a b) : (b = a) := Eq.symm h
+
+
+def add_zero_prop (n: Nat): Prop := n + 0 = n
+-- theorem good (n : Nat) : Prop := Nat.add_zero n
+theorem good (n : Nat) : (add_zero_prop n) := Nat.add_zero n
+
+#check good
+#check Nat.add_zero
+
 end Equality
+
+
+namespace AccessControl
+-- Facts in your system
+variable (User Resource : Type)
+
+-- Policies/claims (propositions)
+variable (CanRead : User → Resource → Prop)
+variable (IsOwner : User → Resource → Prop)
+variable (HasRoleAdmin : User → Prop)
+
+-- Policy rule: owners can read
+variable (owner_rule : ∀ u r, IsOwner u r → CanRead u r)
+
+-- Policy rule: admins can read anything
+variable (admin_rule : ∀ u r, HasRoleAdmin u → CanRead u r)
+
+-- Concrete evidence in one request:
+variable (alice bob : User)
+variable (file1 file2 : Resource)
+variable (hOwner1 : IsOwner alice file1)
+variable (hAdmin : HasRoleAdmin bob)
+
+#check hOwner1
+#check owner_rule
+
+-- Build proof that alice can read file1
+def allow_read_owner : CanRead alice file1 :=
+  owner_rule alice file1 hOwner1
+
+-- Practice: use `admin_rule` with an admin proof.
+def allow_read_admin : CanRead bob file1 :=
+   admin_rule bob file1 hAdmin
+
+-- Practice: combine the two policy paths with case analysis on `Or`.
+theorem allow_read_from_owner_or_admin : CanRead alice file1 :=
+  sorry
+
+axiom owner_rule_a : ∀ (u: User) (r: Resource), IsOwner u r → CanRead u r
+axiom admin_rule_a : ∀ (u: User) (r: Resource), HasRoleAdmin u → CanRead u r
+#check owner_rule_a
+
+theorem allow_read_from_owner_or_admin_any
+    (u : User) (r : Resource)
+    (h : IsOwner u r ∨ HasRoleAdmin u) :
+    CanRead u r :=
+    Or.elim h
+      (fun howner => owner_rule_a User Resource CanRead IsOwner u r howner)
+      (fun hrole => admin_rule_a User Resource CanRead HasRoleAdmin u r hrole)
+
+
+-- Practice: if user can read every resource, then user can read this one.
+theorem allow_read_of_global_access (hAll : ∀ r : Resource, CanRead alice r) : CanRead alice file1 :=
+  hAll file1
+
+end AccessControl
